code/experimental/P256/Hacl.Spec.P256.SolinasReduction.fst
@@ -1,18 +1,50 @@
+
 module Hacl.Spec.P256.SolinasReduction
 
 open Lib.IntTypes 
 open FStar.Math.Lemmas
 open FStar.Math.Lib
 module D = Hacl.Spec.Curve25519.Field64.Definition
+open Hacl.Spec.P256.Definitions
 open FStar.Mul
 open Lib.Sequence
 
 open Hacl.Spec.P256.Core
 
-#reset-options " --z3rlimit 300"
+let _uint32 = n: nat {n < pow2 32}
 
-let prime:pos = pow2 256 - pow2 224 + pow2 192 + pow2 96 -1 
-type _uint32 = a: nat {a < pow2 32}
+inline_for_extraction noextract
+val get_high_part: a: uint64 -> Tot (r: uint32{uint_v r == uint_v a / (pow2 32)})
+
+let get_high_part a = 
+  to_u32(shift_right a (size 32))
+
+
+
+inline_for_extraction noextract
+val get_low_part: a: uint64 -> Tot (r: uint32{uint_v r == uint_v a % (pow2 32)}) 
+
+let get_low_part a = to_u32 a
+
+
+
+val lemma_xor_zero: low: uint64{uint_v (get_high_part low) ==  0} -> high: uint64{uint_v (get_low_part high) == 0} ->  Lemma (uint_v (logxor low high) = uint_v high * pow2 32 + uint_v low)
+
+let lemma_xor_zero low high = 
+  assert(uint_v low = uint_v (get_low_part low));
+  assert(uint_v high = uint_v (get_high_part high) * pow2 32);
+  admit()
+
+val store_high_low_u: high: uint32 -> low: uint32 -> Tot (r: uint64 {uint_v r = uint_v high * pow2 32+ uint_v low})
+
+
+let store_high_low_u high low = 
+  let as_uint64_high = to_u64 high in 
+  let as_uint64_high = Lib.IntTypes.shift_left as_uint64_high (size 32) in 
+  let as_uint64_low = to_u64 low in
+  lemma_xor_zero as_uint64_low as_uint64_high;
+  logxor as_uint64_low as_uint64_high
+
 
 
 val c8_reduction: c8: _uint32  -> 
@@ -230,193 +262,6 @@ let solinas_reduction_mod c0 c1 c2 c3 c4 c5 c6 c7 c8 c9 c10 c11 c12 c13 c14 c15 
   inside_mod1 s0_  s1_ s2_ s3_ s4_ s5_ s6_ s7_ s8_
 
 
-inline_for_extraction noextract
-val fast_reduction_upload_zero_buffer: input: felem8_32 -> Tot (r: felem4
-{
-   let (c0, c1, c2, c3, c4, c5, c6, c7) = input in 
-   let (r0, r1, r2, r3) = r in 
-   D.as_nat4 r == uint_v c0 + uint_v c1 * pow2 (1 * 32) + uint_v c2 * pow2 (2 * 32) + uint_v c3 * pow2 (3 * 32) + uint_v c4 * pow2 (4 * 32) + uint_v c5 * pow2 (5 * 32) + uint_v  c6 * pow2 (6 * 32) + uint_v c7 * pow2 (7 * 32)})
-
-let fast_reduction_upload_zero_buffer (c0, c1, c2, c3, c4, c5, c6, c7)  = 
-  (* let (c0, c1, c2, c3, c4, c5, c6, c7) = input in    *)
-  let b0 = store_high_low_u c1 c0 in 
-  let b1 = store_high_low_u c3 c2 in 
-  let b2 = store_high_low_u c5 c4 in 
-  let b3 = store_high_low_u c7 c6 in 
-  assert_norm (pow2 (1 * 32) * pow2 (2 * 32) = pow2 (3 * 32));
-  assert_norm (pow2 (2 * 32) * pow2 (2 * 32) = pow2 (4 * 32));
-  assert_norm (pow2 (3 * 32) * pow2 (2 * 32) = pow2 (5 * 32));
-  assert_norm (pow2 (4 * 32) * pow2 (2 * 32) = pow2 (6 * 32));
-  assert_norm (pow2 (5 * 32) * pow2 (2 * 32) = pow2 (7 * 32));
-  (b0, b1, b2, b3)
-
-
-inline_for_extraction noextract
-val fast_reduction_upload_first_buffer: input: felem8_32 -> Tot (r: felem4 
-{
-  let (c8, c9, c10, c11, c12, c13, c14, c15) = input in 
-  let (r0, r1, r2, r3) = r in 
-  D.as_nat4 r == (uint_v c11 * pow2 (3 * 32) + uint_v c12 * pow2 (4 * 32) + uint_v c13 * pow2 (5 * 32) + uint_v c14 * pow2 (6 * 32) + uint_v c15 * pow2 (7 * 32)) % prime})
-
-let fast_reduction_upload_first_buffer (c8, c9, c10, c11, c12, c13, c14, c15) = 
-  (* let (c8, c9, c10, c11, c12, c13, c14, c15) = input in  *)
-  let b0 = u64(0) in 
-  let b1 = store_high_low_u c11 (u32 0) in 
-  let b2 = store_high_low_u c13 c12 in 
-  let b3 = store_high_low_u c15 c14 in 
-  assert_norm (pow2 (1 * 32) * pow2 (2 * 32) = pow2 (3 * 32));
-  assert_norm (pow2 (2 * 32) * pow2 (2 * 32) = pow2 (4 * 32));
-  assert_norm (pow2 (3 * 32) * pow2 (2 * 32) = pow2 (5 * 32));
-  assert_norm (pow2 (4 * 32) * pow2 (2 * 32) = pow2 (6 * 32));
-  assert_norm (pow2 (5 * 32) * pow2 (2 * 32) = pow2 (7 * 32));
-  reduction_prime_2prime (b0, b1, b2, b3)
-  
-
-inline_for_extraction noextract
-val fast_reduction_upload_second_buffer: input: felem8_32 -> Tot (r: felem4
-{
-  let (c8, c9, c10, c11, c12, c13, c14, c15) = input in 
-  let (r0, r1, r2, r3) = r in 
-  D.as_nat4 r = (uint_v c12 * pow2 (3 * 32) + uint_v c13 * pow2 (4 * 32) + uint_v c14 * pow2 (5* 32) + uint_v c15 * pow2 (6 * 32)) % prime})
-
-let fast_reduction_upload_second_buffer (c8, c9, c10, c11, c12, c13, c14, c15) = 
-    (* let (c8, c9, c10, c11, c12, c13, c14, c15) = input in  *)
-    let b0 = u64 (0) in 
-    let b1 = store_high_low_u c12 (u32 0) in 
-    let b2 = store_high_low_u c14 c13 in 
-    let b3 = store_high_low_u (u32 0) c15 in 
-      assert_norm (pow2 (1 * 32) * pow2 (2 * 32) = pow2 (3 * 32));
-      assert_norm (pow2 (2 * 32) * pow2 (2 * 32) = pow2 (4 * 32));
-      assert_norm (pow2 (3 * 32) * pow2 (2 * 32) = pow2 (5 * 32));
-      assert_norm (pow2 (4 * 32) * pow2 (2 * 32) = pow2 (6 * 32));
-    (b0, b1, b2, b3)
-
-inline_for_extraction noextract
-val fast_reduction_upload_third_buffer: input: felem8_32 -> Tot (r: felem4
-{
-  let (c8, c9, c10, c11, c12, c13, c14, c15) = input in 
-  let (r0, r1, r2, r3) = r in 
-  D.as_nat4 r = uint_v c8 + uint_v c9 * pow2 32 + uint_v c10 * pow2 (2 * 32) + uint_v c14 * pow2 (6 * 32) + uint_v c15 * pow2 (7 * 32)
-  })
-
-let fast_reduction_upload_third_buffer (c8, c9, c10, c11, c12, c13, c14, c15) = 
-   (* let (c8, c9, c10, c11, c12, c13, c14, c15) = input in  *)
-   let b0 = store_high_low_u c9 c8 in 
-   let b1 = store_high_low_u (u32 0) c10 in 
-   let b2 = u64 0 in 
-   let b3 = store_high_low_u c15 c14 in 
-     assert_norm (pow2 (1 * 32) * pow2 (2 * 32) = pow2 (3 * 32));
-     assert_norm (pow2 (2 * 32) * pow2 (2 * 32) = pow2 (4 * 32));
-     assert_norm (pow2 (3 * 32) * pow2 (2 * 32) = pow2 (5 * 32));
-     assert_norm (pow2 (4 * 32) * pow2 (2 * 32) = pow2 (6 * 32));
-     assert_norm (pow2 (5 * 32) * pow2 (2 * 32) = pow2 (7 * 32));
-   (b0, b1, b2, b3)
-
-inline_for_extraction noextract
-val fast_reduction_upload_forth_buffer: input: felem8_32 -> Tot (r: felem4
-{
-  let (c8, c9, c10, c11, c12, c13, c14, c15) = input in 
-  let (r0, r1, r2, r3) = r in 
-  D.as_nat4 r = uint_v c9 + uint_v c10 * pow2 32 + uint_v c11 * pow2 (2 * 32) + uint_v c13 * pow2 (3 * 32) + uint_v c14 * pow2 (4 * 32) + uint_v c15 * pow2 (5 * 32) + uint_v c13 * pow2 (6 * 32) + uint_v c8 * pow2 (7 * 32)})
-
-let fast_reduction_upload_forth_buffer (c8, c9, c10, c11, c12, c13, c14, c15) = 
-    (* let (c8, c9, c10, c11, c12, c13, c14, c15) = input in  *)
-    let b0 = store_high_low_u c10 c9 in 
-    let b1 = store_high_low_u c13 c11 in 
-    let b2 = store_high_low_u c15 c14 in 
-    let b3 = store_high_low_u c8 c13 in 
-     assert_norm (pow2 (1 * 32) * pow2 (2 * 32) = pow2 (3 * 32));
-     assert_norm (pow2 (2 * 32) * pow2 (2 * 32) = pow2 (4 * 32));
-     assert_norm (pow2 (3 * 32) * pow2 (2 * 32) = pow2 (5 * 32));
-     assert_norm (pow2 (4 * 32) * pow2 (2 * 32) = pow2 (6 * 32));
-     assert_norm (pow2 (5 * 32) * pow2 (2 * 32) = pow2 (7 * 32));
-    (b0, b1, b2, b3)
-
-inline_for_extraction noextract
-val fast_reduction_upload_fifth_buffer: input: felem8_32 -> Tot (r: felem4 
-{
-  let (c8, c9, c10, c11, c12, c13, c14, c15) = input in 
-  let (r0, r1, r2, r3) = r in 
-  D.as_nat4 r = uint_v c11 + uint_v c12 * pow2 32 + uint_v c13 * pow2 (2 * 32) + uint_v c8 * pow2 (6 * 32) + uint_v c10 * pow2 (7 * 32)})
-
-let fast_reduction_upload_fifth_buffer (c8, c9, c10, c11, c12, c13, c14, c15) = 
-    (* let (c8, c9, c10, c11, c12, c13, c14, c15) = input in  *)
-    let b0 = store_high_low_u c12 c11 in 
-    let b1 = store_high_low_u (u32 0) c13 in 
-    let b2 = u64 0 in 
-    let b3 = store_high_low_u c10 c8 in 
-     assert_norm (pow2 (1 * 32) * pow2 (2 * 32) = pow2 (3 * 32));
-     assert_norm (pow2 (2 * 32) * pow2 (2 * 32) = pow2 (4 * 32));
-     assert_norm (pow2 (3 * 32) * pow2 (2 * 32) = pow2 (5 * 32));
-     assert_norm (pow2 (4 * 32) * pow2 (2 * 32) = pow2 (6 * 32));
-     assert_norm (pow2 (5 * 32) * pow2 (2 * 32) = pow2 (7 * 32));
-    (b0, b1, b2, b3)
-
-inline_for_extraction noextract
-val fast_reduction_upload_sixth_buffer: input: felem8_32 -> Tot (r: felem4
-{
-  let (c8, c9, c10, c11, c12, c13, c14, c15) = input in 
-  let (r0, r1, r2, r3) = r in 
-  D.as_nat4 r = uint_v c12 + uint_v c13 * pow2 32 + uint_v c14 * pow2 (2 * 32) + uint_v c15 * pow2 (3 * 32) + 
-      uint_v c9 * pow2 (6 * 32) + uint_v c11 * pow2 (7 * 32)})
-
-let fast_reduction_upload_sixth_buffer (c8, c9, c10, c11, c12, c13, c14, c15) = 
-    (* let (c8, c9, c10, c11, c12, c13, c14, c15) = input in  *)
-    let b0 = store_high_low_u c13 c12 in 
-    let b1 = store_high_low_u c15 c14 in 
-    let b2 = u64 0 in 
-    let b3 = store_high_low_u c11 c9 in 
-     assert_norm (pow2 (1 * 32) * pow2 (2 * 32) = pow2 (3 * 32));
-     assert_norm (pow2 (2 * 32) * pow2 (2 * 32) = pow2 (4 * 32));
-     assert_norm (pow2 (3 * 32) * pow2 (2 * 32) = pow2 (5 * 32));
-     assert_norm (pow2 (4 * 32) * pow2 (2 * 32) = pow2 (6 * 32));
-     assert_norm (pow2 (5 * 32) * pow2 (2 * 32) = pow2 (7 * 32));
-   (b0, b1, b2, b3)
-
-inline_for_extraction noextract
-val fast_reduction_upload_seventh_buffer: input: felem8_32 -> Tot (r: felem4
-{
-  let (c8, c9, c10, c11, c12, c13, c14, c15) = input in 
-  let (r0, r1, r2, r3) = r in 
-  D.as_nat4 r = uint_v c13 + uint_v c14 * pow2 32 + uint_v c15 * pow2 (2 * 32) + uint_v c8 * pow2 (3* 32) +  uint_v c9 * pow2 (4 * 32) + uint_v c10 * pow2 (5 * 32) + uint_v c12 * pow2 (7 * 32)})
-
-
-let fast_reduction_upload_seventh_buffer (c8, c9, c10, c11, c12, c13, c14, c15) = 
-    (* let (c8, c9, c10, c11, c12, c13, c14, c15) = input in  *)
-    let b0 = store_high_low_u c14 c13 in 
-    let b1 = store_high_low_u c8 c15 in 
-    let b2 = store_high_low_u c10 c9 in 
-    let b3 = store_high_low_u c12 (u32 0) in 
-     assert_norm (pow2 (1 * 32) * pow2 (2 * 32) = pow2 (3 * 32));
-     assert_norm (pow2 (2 * 32) * pow2 (2 * 32) = pow2 (4 * 32));
-     assert_norm (pow2 (3 * 32) * pow2 (2 * 32) = pow2 (5 * 32));
-     assert_norm (pow2 (4 * 32) * pow2 (2 * 32) = pow2 (6 * 32));
-     assert_norm (pow2 (5 * 32) * pow2 (2 * 32) = pow2 (7 * 32));
-    (b0, b1, b2, b3)
-
-inline_for_extraction noextract
-val fast_reduction_upload_eighth_buffer: input: felem8_32 -> Tot (r: felem4
-{
-  let (c8, c9, c10, c11, c12, c13, c14, c15) = input in 
-  let (r0, r1, r2, r3) = r in 
-  D.as_nat4 r = uint_v c14 + uint_v c15 * pow2 32 + uint_v c9 * pow2 (3 * 32) + uint_v c10 * pow2 (4* 32) + uint_v c11 * pow2 (5 * 32) + uint_v c13 * pow2 (7 * 32)})
-
-
-let fast_reduction_upload_eighth_buffer (c8, c9, c10, c11, c12, c13, c14, c15) = 
-    (* let (c8, c9, c10, c11, c12, c13, c14, c15) = input in  *)
-    let b0 = store_high_low_u c15 c14 in 
-    let b1 = store_high_low_u c9 (u32 0) in 
-    let b2 = store_high_low_u c11 c10 in 
-    let b3 = store_high_low_u c13 (u32 0) in 
-     assert_norm (pow2 (1 * 32) * pow2 (2 * 32) = pow2 (3 * 32));
-     assert_norm (pow2 (2 * 32) * pow2 (2 * 32) = pow2 (4 * 32));
-     assert_norm (pow2 (3 * 32) * pow2 (2 * 32) = pow2 (5 * 32));
-     assert_norm (pow2 (4 * 32) * pow2 (2 * 32) = pow2 (6 * 32));
-     assert_norm (pow2 (5 * 32) * pow2 (2 * 32) = pow2 (7 * 32));    
-    (b0, b1, b2, b3)
-
-#reset-options " --z3rlimit 300 --z3refresh"
-
 val reduce_brackets: r0: nat -> r1: nat -> r2: nat -> r3: nat -> r4: nat -> r5: nat -> r6: nat -> r7: nat -> r8: nat ->  
   Lemma (
     (((((((((r0 + (2 * r1 % prime)) % prime +  (2 * r2 % prime)) % prime) + r3) % prime + r4) % prime - r5) % prime - r6) % prime - r7) % prime - r8) % prime == 
@@ -447,123 +292,3 @@ let reduce_brackets r0 r1 r2 r3 r4 r5 r6 r7 r8  =
   lemma_mod_add_distr (r0 + t1) (2 * r1 % prime) prime;
   lemma_mod_mul_distr_r 2 r1 prime;
   lemma_mod_add_distr (r0 + t1) (2 * r1) prime
-
-#reset-options " --z3rlimit 200 --z3refresh"
-
-
-let solinas_reduction (f0, f1, f2, f3, f4, f5, f6, f7) = 
-    assert_norm (pow2 64 * pow2 64 = pow2 (2 * 64));
-    assert_norm (pow2 64 * pow2 64 * pow2 64 = pow2 (3 * 64));
-    assert_norm (pow2 64 * pow2 64 * pow2 64 * pow2 64 = pow2 (4 * 64));
-    assert_norm (pow2 64 * pow2 64 * pow2 64 * pow2 64 * pow2 64 = pow2 (5 * 64));
-    assert_norm (pow2 64 * pow2 64 * pow2 64 * pow2 64 * pow2 64 * pow2 64  = pow2 (6 * 64));
-    assert_norm (pow2 64 * pow2 64 * pow2 64 * pow2 64 * pow2 64 * pow2 64 * pow2 64 = pow2 (7 * 64));
-
-    assert(D.wide_as_nat4 (f0, f1, f2, f3, f4, f5, f6, f7) = uint_v f0 + uint_v f1 * pow2 64 + uint_v f2 * pow2 (2 * 64) + uint_v f3 * pow2 (3 * 64) + uint_v f4 * pow2 (4 * 64) + uint_v  f5 * pow2 (5 * 64) + uint_v f6*pow2 (6 * 64) + uint_v f7 * pow2 (7 * 64)); 
-
-  let c0 = get_low_part f0 in 
-  [@inline_let]
-    let c0_n = uint_v c0 in 
-  let c1 = get_high_part f0 in 
-  [@inline_let]
-    let c1_n = uint_v c1 in 
-  let c2 = get_low_part f1 in
-  [@inline_let]
-    let c2_n = uint_v c2 in 
-  let c3 = get_high_part f1 in
-  [@inline_let]
-    let c3_n = uint_v c3 in 
-  let c4 = get_low_part f2 in
-  [@inline_let]
-    let c4_n = uint_v c4 in 
-  let c5 = get_high_part f2 in
-  [@inline_let]
-    let c5_n = uint_v c5 in 
-  let c6 = get_low_part f3 in
-  [@inline_let]
-    let c6_n = uint_v c6 in 
-  let c7 = get_high_part f3 in
-  [@inline_let]
-    let c7_n = uint_v c7 in 
-  let c8 = get_low_part f4 in 
-  [@inline_let]
-    let c8_n = uint_v c8 in 
-  let c9 = get_high_part f4 in
-  [@inline_let]
-    let c9_n = uint_v c9 in
-  let c10 = get_low_part f5 in   
-  [@inline_let]
-    let c10_n = uint_v c10 in 
-  let c11 = get_high_part f5 in
-  [@inline_let]
-    let c11_n = uint_v c11 in 
-  let c12 = get_low_part f6 in 
-  [@inline_let]
-    let c12_n = uint_v c12 in 
-  let c13 = get_high_part f6 in
-  [@inline_let]
-    let c13_n = uint_v c13 in 
-  let c14 = get_low_part  f7 in
-  [@inline_let]
-    let c14_n = uint_v c14 in 
-  let c15 = get_high_part f7 in
-  [@inline_let]
-    let c15_n = uint_v c15 in
-
-  assert_norm (pow2 (1 * 32) * pow2 (2 * 32) = pow2 (3 * 32));
-  assert_norm (pow2 (2 * 32) * pow2 (2 * 32) = pow2 (4 * 32));
-  assert_norm (pow2 (3 * 32) * pow2 (2 * 32) = pow2 (5 * 32));
-  assert_norm (pow2 (4 * 32) * pow2 (2 * 32) = pow2 (6 * 32));
-  assert_norm (pow2 (5 * 32) * pow2 (2 * 32) = pow2 (7 * 32));
-  assert_norm (pow2 (6 * 32) * pow2 (2 * 32) = pow2 (8 * 32));
-  assert_norm (pow2 (7 * 32) * pow2 (2 * 32) = pow2 (9 * 32));
-  assert_norm (pow2 (8 * 32) * pow2 (2 * 32) = pow2 (10 * 32));
-  assert_norm (pow2 (9 * 32) * pow2 (2 * 32) = pow2 (11 * 32));
-  assert_norm (pow2 (10 * 32) * pow2 (2 * 32) = pow2 (12 * 32));
-  assert_norm (pow2 (11 * 32) * pow2 (2 * 32) = pow2 (13 * 32));
-  assert_norm (pow2 (12 * 32) * pow2 (2 * 32) = pow2 (14 * 32));
-  assert_norm (pow2 (13 * 32) * pow2 (2 * 32) = pow2 (15 * 32)); 
-
-  assert(D.wide_as_nat4 (f0, f1, f2, f3, f4, f5, f6, f7) =  (c0_n + c1_n * pow2 32 + c2_n * pow2 (2 * 32) + c3_n * pow2 (3 * 32) + c4_n * pow2 (4 * 32) + c5_n * pow2 (5 * 32) + c6_n * pow2 (6 * 32) + c7_n * pow2 (7 * 32) + c8_n * pow2 256 + c9_n * pow2 288 + c10_n * pow2 (10 * 32)  + c11_n * pow2 (11 * 32) + c12_n * pow2 (12 * 32) + c13_n* pow2 (13 * 32) + c14_n * pow2 (14 * 32) + c15_n * pow2 (15 * 32)));
-
-  (* let c_low = (c0, c1, c2, c3, c4, c5, c6, c7) in  *)
-  (* let c_high = (c8, c9, c10, c11, c12, c13, c14, c15) in  *)
-
-  let (state0_0, state0_1, state0_2, state0_3) = fast_reduction_upload_zero_buffer  (c0, c1, c2, c3, c4, c5, c6, c7) in 
-    let (state0_red_0, state0_red_1, state0_red_2, state0_red_3) = reduction_prime_2prime (state0_0, state0_1, state0_2, state0_3) in 
-  let state1 = fast_reduction_upload_first_buffer (c8, c9, c10, c11, c12, c13, c14, c15) in 
-  let state2 = fast_reduction_upload_second_buffer (c8, c9, c10, c11, c12, c13, c14, c15) in 
-  let state3 = fast_reduction_upload_third_buffer (c8, c9, c10, c11, c12, c13, c14, c15) in 
-      let state3_red = reduction_prime_2prime state3 in 
-  let state4 = fast_reduction_upload_forth_buffer (c8, c9, c10, c11, c12, c13, c14, c15) in 
-      let state4_red = reduction_prime_2prime state4 in 
-  let state5 = fast_reduction_upload_fifth_buffer (c8, c9, c10, c11, c12, c13, c14, c15) in
-      let state5_red = reduction_prime_2prime state5 in     
-  let state6 = fast_reduction_upload_sixth_buffer (c8, c9, c10, c11, c12, c13, c14, c15) in 
-    let state6_red = reduction_prime_2prime state6 in 
-  let state7 = fast_reduction_upload_seventh_buffer (c8, c9, c10, c11, c12, c13, c14, c15) in 
-      let state7_red = reduction_prime_2prime state7 in 
-  let state8 = fast_reduction_upload_eighth_buffer (c8, c9, c10, c11, c12, c13, c14, c15) in 
-      let state8_red = reduction_prime_2prime state8 in 
-
-  let state1_2 = shift_left_felem state1 in 
-  let state2_2 = shift_left_felem state2 in 
-  let r0 = felem_add (state0_red_0, state0_red_1, state0_red_2, state0_red_3)  state1_2 in 
-  let r1 = felem_add r0 state2_2 in 
-  let r0 = felem_add r1 state3_red in 
-  let r1 = felem_add r0 state4_red in 
-  let r0 = felem_sub r1 state5_red in 
-  let r1 = felem_sub r0 state6_red in 
-  let r0 = felem_sub r1 state7_red in 
-  let result = felem_sub r0 state8_red in 
-    modulo_lemma (D.as_nat4 result) prime;
-
-  reduce_brackets (D.as_nat4 (state0_red_0, state0_red_1, state0_red_2, state0_red_3) ) (D.as_nat4 state1) (D.as_nat4 state2) (D.as_nat4 state3_red) (D.as_nat4 state4_red) (D.as_nat4 state5_red) (D.as_nat4 state6_red) (D.as_nat4 state7_red) (D.as_nat4 state8_red);
-
-  solinas_reduction_mod c0_n c1_n c2_n c3_n c4_n c5_n c6_n c7_n c8_n c9_n c10_n c11_n c12_n c13_n c14_n c15_n 
-    (D.as_nat4 (state0_red_0, state0_red_1, state0_red_2, state0_red_3) ) (D.as_nat4 state1) (D.as_nat4 state2) (D.as_nat4 state3_red) 
-    (D.as_nat4 state4_red) (D.as_nat4 state5_red) (D.as_nat4 state6_red) (D.as_nat4 state7_red)
-    (D.as_nat4  state8_red) (D.as_nat4 result);
-
- result
-
